NuPrime.thy
@@ -231,9 +231,9 @@ subsubsection \<open>Properties\<close>
 
 definition \<nu>Zero :: "('a::{zero,lrep},'b) \<nu> \<Rightarrow> 'b \<Rightarrow> bool"
   where [\<nu>def]: "\<nu>Zero N x \<longleftrightarrow> (\<forall>res. [res] 0 \<nuLinkL> N \<nuLinkR> x )"
-definition \<nu>Equal :: "('a::{lrep,ceq}, 'b) \<nu> \<Rightarrow> (heap \<Rightarrow> 'b \<Rightarrow> 'b \<Rightarrow> bool) \<Rightarrow> ('b \<Rightarrow> 'b \<Rightarrow> bool) \<Rightarrow> bool"
+definition \<nu>Equal :: "('a::{lrep,ceq}, 'b) \<nu> \<Rightarrow> ('b \<Rightarrow> 'b \<Rightarrow> bool) \<Rightarrow> ('b \<Rightarrow> 'b \<Rightarrow> bool) \<Rightarrow> bool"
   where [\<nu>def]: "\<nu>Equal N can_eq eq \<longleftrightarrow> (\<forall>p1 p2 x1 x2 heap.
-    ceqable heap p1 p2 \<and> ([heap] p1 \<nuLinkL> N \<nuLinkR> x1) \<and> ([heap] p2 \<nuLinkL> N \<nuLinkR> x2) \<longrightarrow> can_eq heap x1 x2 \<and> (ceq p1 p2 = eq x1 x2))"
+    ceqable heap p1 p2 \<and> ([heap] p1 \<nuLinkL> N \<nuLinkR> x1) \<and> ([heap] p2 \<nuLinkL> N \<nuLinkR> x2) \<longrightarrow> can_eq x1 x2 \<and> (ceq p1 p2 = eq x1 x2))"
 
 definition \<nu>Resources_of_set :: " 'a \<nu>set \<Rightarrow> resource_key set \<Rightarrow> bool "
   where [\<nu>def]: "\<nu>Resources_of_set S rcss \<longleftrightarrow> (\<forall>heap adr v p. adr \<notin> rcss \<longrightarrow> p \<in> S heap \<longrightarrow> p \<in> S (heap(adr := v)))"
@@ -286,7 +286,7 @@ definition Premise :: "bool \<Rightarrow> bool" ("\<^bold>p\<^bold>r\<^bold>e\<^
 lemma Premise_I: "P \<Longrightarrow> \<^bold>p\<^bold>r\<^bold>e\<^bold>m\<^bold>i\<^bold>s\<^bold>e P" unfolding Premise_def by simp
 lemma Premise_E: "\<^bold>p\<^bold>r\<^bold>e\<^bold>m\<^bold>i\<^bold>s\<^bold>e P \<Longrightarrow> P" unfolding Premise_def by simp
 lemma [elim!,\<nu>elim]: "\<^bold>p\<^bold>r\<^bold>e\<^bold>m\<^bold>i\<^bold>s\<^bold>e P \<Longrightarrow> (P \<Longrightarrow> C) \<Longrightarrow> C" unfolding Premise_def by simp
-lemma Premise_Irew: "(P \<Longrightarrow> PROP C) \<equiv> (\<^bold>p\<^bold>r\<^bold>e\<^bold>m\<^bold>i\<^bold>s\<^bold>e P \<Longrightarrow> PROP C)" unfolding Premise_def by simp
+lemma Premise_Irew: "(P \<Longrightarrow> C) \<equiv> Trueprop (\<^bold>p\<^bold>r\<^bold>e\<^bold>m\<^bold>i\<^bold>s\<^bold>e P \<longrightarrow> C)" unfolding Premise_def atomize_imp .
 
 (* attribute_setup intro_premise = \<open>
   Scan.succeed (Thm.rule_attribute [] (fn _ => fn th => th COMP @{thm Premise_I}))
